checker/src/g_metacoq_checker.ml4
@@ -15,7 +15,7 @@ let check env evm c =
   let term = Ast_quoter.quote_term_rec env (EConstr.to_constr evm c) in
   (* Feedback.msg_debug (str"Finished quoting.. checking."); *)
   let fuel = pow two (pow two (pow two two)) in
-  let checker_flags = true in
+  let checker_flags = Config0.default_checker_flags in
   match Checker0.typecheck_program checker_flags fuel term with
   | CorrectDecl t ->
      Feedback.msg_info (str "Successfully checked of type: " ++ pr_char_list (Checker0.string_of_term t))
